Started logically-atomic get for top-level clerk;
need to regoose to fix some messed up loop translations

src/program_proof/memkv/common_proof.v
@@ -4,6 +4,18 @@ From Perennial.goose_lang Require Import ffi.grove_ffi.
 
 Section common_proof.
 
+Context `{!heapG Σ}.
 
+Definition uNSHARD : nat := 65536.
+Lemma wp_shardOf_bound (key:u64) :
+  {{{
+      True
+  }}}
+    shardOf #key
+  {{{
+     (s:u64), RET #s; ⌜((int.nat s) < uNSHARD)%nat⌝
+  }}}.
+Proof.
+Admitted.
 
 End common_proof.
