src/program_proof/memkv/memkv_clerk_proof.v
@@ -1,0 +1,105 @@
+From Perennial.program_proof Require Import proof_prelude.
+From Goose.github_com.mit_pdos.gokv Require Import memkv.
+From Perennial.goose_lang Require Import ffi.grove_ffi.
+From Perennial.program_proof.lockservice Require Import rpc.
+From Perennial.program_proof.memkv Require Import common_proof memkv_coord_clerk_proof memkv_shard_clerk_proof.
+
+Section memkv_clerk_proof.
+
+Context `{!heapG Σ, rpcG Σ GetReplyC}.
+
+Definition own_MemKVClerk (ck:loc) (γ:gname) : iProp Σ :=
+  ∃ (s coordCk:loc) shardMap_sl (shardMapping:list u64),
+  "HshardClerks" ∷ ck ↦[MemKVClerk.S :: "shardClerks"] #s ∗
+  "HshardClerksSet" ∷ own_ShardClerkSet s γ ∗
+  "HcoordCk" ∷ ck ↦[MemKVClerk.S :: "coordCk"] #coordCk ∗
+  "HcoordCk_own" ∷ own_MemKVCoordClerk coordCk ∗
+  "HshardMap" ∷ ck ↦[MemKVClerk.S :: "shardMap"] (slice_val shardMap_sl) ∗
+  "HshardMap_sl" ∷ typed_slice.is_slice shardMap_sl uint64T 1%Qp shardMapping ∗
+  "%HshardMap_length" ∷ ⌜length shardMapping = uNSHARD⌝
+.
+
+Lemma KVClerk__Get Eo Ei (ck:loc) (γ:gname) (key:u64) :
+  ∀ Φ,
+  own_MemKVClerk ck γ -∗
+  (|={Eo,Ei}=> (∃ v, kvptsto γ key v ∗ (kvptsto γ key v ={Ei,Eo}=∗ (∀ val_sl, typed_slice.is_slice val_sl byteT 1%Qp v -∗ (Φ (slice_val val_sl)))))) -∗
+    WP MemKVClerk__Get #ck #key {{ Φ }}
+.
+Proof.
+  iIntros (Φ) "Hown Hatomic".
+  wp_lam.
+  wp_pures.
+  wp_apply wp_ref_of_zero.
+  { done. }
+  iIntros (rep_ptr) "Hrep".
+  wp_pures.
+
+  iAssert (∃ rep_sl, rep_ptr ↦[slice.T byteT] (slice_val rep_sl) )%I with "[Hrep]" as "Hrep".
+  {
+    iExists _; iFrame.
+    admit.
+  }
+
+  wp_forBreak.
+  wp_pures.
+
+  wp_apply (wp_shardOf_bound).
+  iIntros (sid ?).
+  wp_pures.
+
+  iNamed "Hown".
+  wp_loadField.
+  iDestruct (typed_slice.is_slice_small_acc with "HshardMap_sl") as "[Hsmall_sl HslClose]".
+
+  rewrite -HshardMap_length in H0.
+  eapply list_lookup_lt in H0.
+  destruct H0 as [hostID H0].
+  wp_apply (typed_slice.wp_SliceGet (V:=u64) with "[$Hsmall_sl]").
+  {
+    iPureIntro.
+    done.
+  }
+  iIntros "Hsmall_sl".
+  wp_pures.
+  (* FIXME: need to pass config around to map hostIDs to strings *)
+  wp_loadField.
+  wp_apply (wp_ShardClerkSet__getClerk with "[$HshardClerksSet]").
+  iIntros (??) "(HshardCk & %Hre & HcloseShardSet)".
+
+  wp_pures.
+  wp_apply (wp_MemKVShardClerk__Get Eo Ei γsh with "[Hatomic $HshardCk $Hrep]").
+  {
+    rewrite Hre.
+    iFrame "Hatomic".
+  }
+  iIntros (e) "HshardGetPost".
+  wp_pures.
+  wp_if_destruct.
+  {
+    wp_loadField.
+    iDestruct "HshardGetPost" as "(HshardCk & [Hatomic|[%Hbad _]])"; last first.
+    {
+      exfalso. done.
+    }
+    iDestruct ("HcloseShardSet" with "HshardCk") as "HshardSet".
+    wp_apply (wp_MemKVCoordClerk__GetShardMap with "[$HcoordCk_own]").
+    iIntros (shardMap_sl' shardMapping') "[HcoordCk_own HshardMap_sl]".
+    wp_apply (wp_storeField with "HshardMap").
+    { apply slice_val_ty. }
+    iIntros "HshardMap".
+    wp_pures.
+    iLeft.
+    iModIntro.
+
+    iSplitL ""; first done.
+    iDestruct "Hatomic" as "[_ $]".
+    iExists _,_,_,_; iFrame.
+  }
+  {
+    wp_pures.
+    wp_if_destruct.
+    {
+      wp_pures.
+Admitted.
+
+End memkv_clerk_proof.
