src/program_proof/memkv/memkv_coord_clerk_proof.v
@@ -1,0 +1,44 @@
+From Perennial.program_proof Require Import proof_prelude.
+From Goose.github_com.mit_pdos.gokv Require Import memkv.
+From Perennial.goose_lang Require Import ffi.grove_ffi.
+From Perennial.program_proof.lockservice Require Import rpc.
+From Perennial.program_proof.memkv Require Import common_proof memkv_shard_clerk_proof.
+
+Section memkv_coord_clerk_proof.
+
+Context `{!heapG Σ, rpcG Σ GetReplyC}.
+
+Axiom own_MemKVCoordClerk : loc → iProp Σ.
+
+Lemma wp_MemKVCoordClerk__GetShardMap (ck:loc) :
+  {{{
+       own_MemKVCoordClerk ck
+  }}}
+    MemKVCoordClerk__GetShardMap #ck
+  {{{
+       shardMap_sl (shardMapping:list u64), RET (slice_val shardMap_sl);
+       own_MemKVCoordClerk ck ∗
+       typed_slice.is_slice shardMap_sl uint64T 1%Qp shardMapping ∗
+       ⌜length shardMapping = uNSHARD⌝
+  }}}
+.
+Proof.
+Admitted.
+
+Axiom own_ShardClerkSet : loc → gname → iProp Σ.
+
+(* TODO: need precondition that [[is_shard_server host]] *)
+Lemma wp_ShardClerkSet__getClerk (γkv:gname) (s:loc) (host:u64) :
+  {{{
+       own_ShardClerkSet s γkv
+  }}}
+    ShardClerkSet__getClerk #s #host
+  {{{
+       (ck_ptr:loc) γsh, RET #ck_ptr; own_MemKVShardClerk ck_ptr γsh ∗
+                                      ⌜γsh.(kv_gn) = γkv⌝ ∗
+                                    (own_MemKVShardClerk ck_ptr γsh -∗ own_ShardClerkSet s γkv)
+  }}}.
+Proof.
+Admitted.
+
+End memkv_coord_clerk_proof.
